pulse/share/steel/examples/pulse/dice/engine/EngineCore.fsti
@@ -22,7 +22,10 @@ module U8 = FStar.UInt8
 module SZ = FStar.SizeT
 open HACL
 
+noextract
 val l0_is_authentic (repr:engine_record_repr) : prop
+
+noextract
 val cdi_functional_correctness (c0:Seq.seq U8.t) (uds_bytes:Seq.seq U8.t) (repr:engine_record_repr) : prop 
 
 val engine_main (cdi:A.larray U8.t (SZ.v (digest_len dice_hash_alg))) (uds:A.larray U8.t (SZ.v uds_len)) (record:engine_record_t)
@@ -30,13 +33,14 @@ val engine_main (cdi:A.larray U8.t (SZ.v (digest_len dice_hash_alg))) (uds:A.lar
                 (#repr:Ghost.erased engine_record_repr)
                 (#uds_perm #p:perm)
                 (#uds_bytes:Ghost.erased (Seq.seq U8.t))
-  : stt dice_return_code (engine_record_perm record p repr **
-                          A.pts_to uds #uds_perm uds_bytes **
-                          A.pts_to cdi c0)
-                         (fun r -> 
-                            engine_record_perm record p repr **
-                            A.pts_to uds #uds_perm uds_bytes **
-                            (exists* (c1:Seq.seq U8.t).
-                                      A.pts_to cdi c1 **
-                                      pure (r = DICE_SUCCESS ==>
-                                            l0_is_authentic repr /\ cdi_functional_correctness c1 uds_bytes repr)))
+  : stt (engine_record_t & dice_return_code)
+        (engine_record_perm record p repr **
+         A.pts_to uds #uds_perm uds_bytes **
+         A.pts_to cdi c0)
+        (fun r ->
+         engine_record_perm (fst r) p repr **
+         A.pts_to uds #uds_perm uds_bytes **
+         (exists* (c1:Seq.seq U8.t).
+          A.pts_to cdi c1 **
+          pure (snd r = DICE_SUCCESS ==>
+                l0_is_authentic repr /\ cdi_functional_correctness c1 uds_bytes repr)))
